@prefix dc: <http://purl.org/dc/elements/1.1/> .
@prefix mod: <https://w3id.org/mod#> .
@prefix owl: <http://www.w3.org/2002/07/owl#> .
@prefix rdfs: <http://www.w3.org/2000/01/rdf-schema#> .
@prefix sense: <http://w3id.org/explainability/sense#> .
@prefix sosa: <http://www.w3.org/ns/sosa/> .
@prefix vann: <http://purl.org/vocab/vann/> .
@prefix xsd: <http://www.w3.org/2001/XMLSchema#> .

dc:contributor a owl:AnnotationProperty .

dc:created a owl:AnnotationProperty .

dc:creator a owl:AnnotationProperty .

dc:description a owl:AnnotationProperty .

dc:license a owl:AnnotationProperty .

dc:modified a owl:AnnotationProperty .

dc:title a owl:AnnotationProperty .

sense: a owl:Ontology ;
    dc:contributor "Gernot Steindl",
        "Ioan Toma",
        "Marta Sabou",
        "Mohammad Bilal",
        "Simon Steyskal",
        "Thomas Fr√ºhwirth" ;
    dc:created "2023-11-01" ;
    dc:creator "Fajar J. Ekaputra",
        "Katrin Schreiberhuber" ;
    dc:description "An ontology to create an explainable Cyber Physical System (CPS)"@en ;
    dc:license <https://creativecommons.org/licenses/by/4.0> ;
    dc:modified "2024-10-16" ;
    dc:title "SENSE Ontology",
        "SENSE Ontology"@en ;
    vann:preferredNamespacePrefix "s" ;
    vann:preferredNamespaceUri "http://w3id.org/explainability/sense#" ;
    owl:imports sosa:,
        <https://www.w3.org/ns/ssn/> ;
    owl:versionInfo "3.0" ;
    mod:createdWith <https://chowlk.linkeddata.es/> .

sense:PlatformOfInterest rdfs:comment "A plaform, which can host sensors, but is also a feature of interest." .

sense:ResultType rdfs:comment "A type of Result. This is usually a State Type or an Event Type." .

sense:allowsControlAccessTo a owl:ObjectProperty ;
    rdfs:label "allows control access to" ;
    rdfs:comment "each access right defines access to a certain platform of the system. Access to this plaform means access to all sensors hosted by this platform. ontrol access rights define which parts of the system can be manipulated by this user role." ;
    rdfs:domain sense:AccessRight ;
    rdfs:range sense:Platform .

sense:allowsViewAccessTo a owl:ObjectProperty ;
    rdfs:label "allows view access to" ;
    rdfs:comment "each access right defines access to a certain platform of the system. Access to this plaform means access to all sensors hosted by this platform. View access rights define, which parts of the system can be viewed/contained in an explanation for this user role." ;
    rdfs:domain sense:AccessRight ;
    rdfs:range sense:Platform .

sense:associatedPlatformType a owl:ObjectProperty ;
    rdfs:label "associated platform type" ;
    rdfs:comment "each result type can only be detected at a specified platform type, the associated platform type." ;
    rdfs:domain sense:EventType ;
    rdfs:range sense:PlatformType .

sense:associatedProperty a owl:ObjectProperty ;
    rdfs:label "associated property" ;
    rdfs:comment "Each result type is detected by measurement of an observable Property, its associated Property." ;
    rdfs:domain sense:EventType ;
    rdfs:range sense:ObservableProperty .

sense:bindsToLiteral a owl:DatatypeProperty ;
    rdfs:label "binds to literal" ;
    rdfs:comment "Relation between a ParameterBinding and the literal to which it should bind to. Example: '5' could bind a value in a formula to the literal 5." ;
    rdfs:domain sense:ParameterBinding ;
    rdfs:range xsd:string .

sense:bindsToSensor a owl:ObjectProperty ;
    rdfs:label "binds to sensor" ;
    rdfs:comment "Relation between a ParameterBinding and the sensor to which it should bind." ;
    rdfs:domain sense:ParameterBinding ;
    rdfs:range sense:Sensor .

sense:causalRelation a owl:DatatypeProperty ;
    rdfs:label "causal relation" ;
    rdfs:comment "A type of causal relation, which can be one of three options: causes, prevents, enables" ;
    rdfs:domain sense:StateTypeCausality ;
    rdfs:range xsd:string .

sense:cause a owl:ObjectProperty ;
    rdfs:label "cause" ;
    rdfs:comment "Relation between a state type causality and the state type that is the cause of the relation." ;
    rdfs:domain sense:StateCausality,
        sense:StateTypeCausality ;
    rdfs:range sense:State,
        sense:StateType .

sense:considersAccessRights a owl:ObjectProperty ;
    rdfs:label "considers access rights" ;
    rdfs:comment "Which access rights are considered in the explanation." ;
    rdfs:domain sense:Explanation ;
    rdfs:range sense:AccessRight .

sense:considersUserType a owl:ObjectProperty ;
    rdfs:label "considers user type" ;
    rdfs:comment "The technicality level, which is considered by an explanation." ;
    rdfs:domain sense:Explanation ;
    rdfs:range sense:UserType .

sense:containsAccessRights a owl:ObjectProperty ;
    rdfs:label "contains access rights" ;
    rdfs:comment "Each user role is connected to a set of access rights." ;
    rdfs:domain sense:UserRole ;
    rdfs:range sense:AccessRight .

sense:containsMitigationOption a owl:ObjectProperty ;
    rdfs:label "contains mitigation option" ;
    rdfs:comment "a list of mitigation options, contained in the mitigation plan." ;
    rdfs:domain sense:MitigationPlan ;
    rdfs:range sense:MitigationOption .

sense:dataSource a owl:DatatypeProperty ;
    rdfs:label "data source" ;
    rdfs:comment "reference to the time series data that is collected by a Sensor." ;
    rdfs:domain sense:Sensor ;
    rdfs:range xsd:string .

sense:definition a owl:DatatypeProperty ;
    rdfs:label "definition" ;
    rdfs:comment "Relation between an EventDetection procedure and the definition of what causes an event. The syntax and semantics of the definition depend on the employed method." ;
    rdfs:domain sense:EventDetection ;
    rdfs:range xsd:string .

sense:designedFor a owl:ObjectProperty ;
    rdfs:label "designed for" ;
    rdfs:comment "The user, for whom the explanation is designed." ;
    rdfs:domain sense:Explanation ;
    rdfs:range sense:User .

sense:detectedBy rdfs:comment "each event type is detected by an event detection method." .

sense:detectedEvent a owl:ObjectProperty ;
    rdfs:label "detected event" ;
    rdfs:comment "subproperty of sosa:hasResult - relation from an Observation to its result" ;
    rdfs:domain sense:Observation ;
    rdfs:range sense:Event .

sense:detectsEventType a owl:ObjectProperty ;
    rdfs:label "detects event type" ;
    rdfs:comment "relation from an Event Detection Procedure to the type of event it is designed to detect." ;
    rdfs:domain sense:EventDetection ;
    rdfs:range sense:EventType .

sense:effect a owl:ObjectProperty ;
    rdfs:label "effect" ;
    rdfs:comment "Relation between a state type causality and the state type that is the effect of the relation." ;
    rdfs:domain sense:StateCausality,
        sense:StateTypeCausality ;
    rdfs:range sense:State,
        sense:StateType .

sense:endsStateType a owl:ObjectProperty ;
    rdfs:label "ends state type" ;
    rdfs:comment "inverse of hasEndEventType, relation from an Event to the state ended by the event." ;
    rdfs:domain sense:EventType ;
    rdfs:range sense:StateType ;
    owl:inverseOf sense:hasEndEventType .

sense:eventTime a owl:DatatypeProperty ;
    rdfs:label "event time" ;
    rdfs:comment "Timestamp of when the event is happening." .

sense:explains a owl:ObjectProperty ;
    rdfs:label "explains" ;
    rdfs:comment "The state, which is explained by an explanation." ;
    rdfs:domain sense:Explanation ;
    rdfs:range sense:State .

sense:hasCausalSource a owl:ObjectProperty ;
    rdfs:label "has causal source" ;
    rdfs:comment "An RDF-star relation from a causallyRelated-triple to the state type causality, which is responsible for the causal relation." ;
    rdfs:domain sense:StateCausality ;
    rdfs:range sense:StateTypeCausality .

sense:hasEndEvent a owl:ObjectProperty ;
    rdfs:label "has end event" ;
    rdfs:comment "relation between a state and the event that is ending the state." ;
    rdfs:domain sense:State ;
    rdfs:range sense:Event .

sense:hasFeatureOfInterest a owl:ObjectProperty ;
    rdfs:label "has feature of interest" ;
    rdfs:comment "subclass of sosa:hasFeatureOfInterest -  relation from an Execution to its subject entity" ;
    rdfs:domain sense:Observation ;
    rdfs:range sense:Platform .

sense:hasMitigationPlan a owl:ObjectProperty ;
    rdfs:label "has mitigation plan" ;
    rdfs:comment "each state type has a mitigation plan, which contains a list of mitigation options of a certain state type." ;
    rdfs:domain sense:StateType ;
    rdfs:range sense:MitigationPlan .

sense:hasParameterBinding a owl:ObjectProperty ;
    rdfs:label "has parameter binding" ;
    rdfs:comment "Relation between the EventDetection procedure and a ParameterBinding." ;
    rdfs:domain sense:EventDetection ;
    rdfs:range sense:ParameterBinding .

sense:hasPlatformType rdfs:comment "A relation between a Plaform and its Platformtype." .

sense:hasProperty a owl:ObjectProperty ;
    rdfs:label "has property" ;
    rdfs:comment "Each Plaformtype has observable properties, which can be observed. These properties are defining the states of a feature of interest." ;
    rdfs:domain sense:PlatformType ;
    rdfs:range sense:ObservableProperty .

sense:hasResultType rdfs:comment "each Result has a result type." .

sense:hasStartEvent a owl:ObjectProperty ;
    rdfs:label "has start event" ;
    rdfs:comment "relation between a state and the event that is starting the state." ;
    rdfs:domain sense:State ;
    rdfs:range sense:Event .

sense:hasUnit a owl:DatatypeProperty ;
    rdfs:label "has unit" ;
    rdfs:comment "subclass of qudt:Unit - This property relates a system of units with a unit of measure that is either:" .

sense:hasUserRole a owl:ObjectProperty ;
    rdfs:label "has user role" ;
    rdfs:comment "relation from a user to their user role." ;
    rdfs:domain sense:User ;
    rdfs:range sense:UserRole .

sense:hasUserType a owl:ObjectProperty ;
    rdfs:label "has user type" ;
    rdfs:comment "relation from a user to their user." ;
    rdfs:domain sense:User ;
    rdfs:range sense:UserType .

sense:interestedIn a owl:ObjectProperty ;
    rdfs:label "interested in" ;
    rdfs:comment "A relation from a user to the state types a user is interested in." ;
    rdfs:domain sense:User ;
    rdfs:range sense:StateType .

sense:isHostedBy a owl:ObjectProperty ;
    rdfs:label "is hosted by" ;
    rdfs:comment "inverse relation of sense:hosts." ;
    rdfs:domain sense:Sensor ;
    rdfs:range sense:Platform ;
    owl:inverseOf sense:hosts .

sense:isOfType a owl:ObjectProperty ;
    rdfs:label "is of type" ;
    rdfs:comment "relation from an instance of a class to its class type via explicit typing." ;
    rdfs:domain sense:Event,
        sense:Platform,
        sense:State ;
    rdfs:range sense:EventType,
        sense:PlatformType,
        sense:StateType .

sense:isTriggerStateType a owl:DatatypeProperty ;
    rdfs:label "is trigger state type" ;
    rdfs:comment "A boolean value, whether a StateType is interesting to trigger and explanation." ;
    rdfs:domain sense:StateType ;
    rdfs:range xsd:boolean .

sense:linkedToSensor a owl:ObjectProperty ;
    rdfs:label "linked to sensor" ;
    rdfs:comment "It defines, which sensor measurements are needed to calculate the data of a virtual sensor." ;
    rdfs:domain sense:VirtualSensor ;
    rdfs:range sense:Sensor .

sense:madeObservation a owl:ObjectProperty ;
    rdfs:label "made observation" ;
    rdfs:comment "subclass of sosa:madeObservation -  relation from a Sensor to an Observation or ObservationCollection it has made." ;
    rdfs:domain sense:Sensor ;
    rdfs:range sense:Observation .

sense:method a owl:DatatypeProperty ;
    rdfs:label "method" ;
    rdfs:comment "Relation between the EventDetection procedure and the employed event specification method. This specification method affects the syntax and semantics of the associated definition." ;
    rdfs:domain sense:EventDetection ;
    rdfs:range xsd:string .

sense:observedProperty a owl:ObjectProperty ;
    rdfs:label "observed property" ;
    rdfs:comment "subclass of sosa:observedProperty - relation from an Observation or ObservationCollection to the property that was observed" ;
    rdfs:domain sense:Observation ;
    rdfs:range sense:ObservableProperty .

sense:observes a owl:ObjectProperty ;
    rdfs:label "observes" ;
    rdfs:comment "subclass of sosa:observes -  relation from a Sensor to a Property that it is capable of sensing" ;
    rdfs:domain sense:Sensor .

sense:origin a owl:DatatypeProperty ;
    rdfs:label "origin" ;
    rdfs:comment "The formula needed to calculated the measurements of a virtual sensor." ;
    rdfs:domain sense:VirtualSensor ;
    rdfs:range xsd:string .

sense:parameterName a owl:DatatypeProperty ;
    rdfs:label "parameter name" ;
    rdfs:comment "Relation between a ParameterBinding and its name." ;
    rdfs:domain sense:ParameterBinding ;
    rdfs:range xsd:string .

sense:startsStateType a owl:ObjectProperty ;
    rdfs:label "starts state type" ;
    rdfs:comment "inverse of hasStartEventType, relation from an Event to the state started by the event." ;
    rdfs:domain sense:EventType ;
    rdfs:range sense:StateType ;
    owl:inverseOf sense:hasStartEventType .

sense:suggests a owl:ObjectProperty ;
    rdfs:label "suggests" ;
    rdfs:comment "Mitigation options, which are suggested by an explanation based on a user control access rights." ;
    rdfs:domain sense:Explanation ;
    rdfs:range sense:MitigationOption .

sense:temporalRelation a owl:DatatypeProperty ;
    rdfs:label "temporal relation" ;
    rdfs:comment "A type of temporal relation, which can be one of four options: before, overlaps, contains, identity" ;
    rdfs:domain sense:StateTypeCausality ;
    rdfs:range xsd:string .

sense:topologicalRelation a owl:DatatypeProperty ;
    rdfs:label "topological relation" ;
    rdfs:comment "A type of topological relation, which can be one of three options: samePlatform, siblingPlatform, parentPlatform" ;
    rdfs:domain sense:StateTypeCausality ;
    rdfs:range xsd:string .

sense:usedProcedure a owl:ObjectProperty ;
    rdfs:label "used procedure" ;
    rdfs:comment "subclass of sosa:usedProcedure - relation from an Execution to a Procedure used to make it" ;
    rdfs:domain sense:Observation ;
    rdfs:range sense:EventDetection .

owl:versionInfo a owl:AnnotationProperty .

sense:hasEndEventType a owl:ObjectProperty ;
    rdfs:label "has end event type" ;
    rdfs:comment "Relation between a state type and an event type. Describes which event type ends a certain state type." ;
    rdfs:domain sense:StateType ;
    rdfs:range sense:EventType .

sense:hasStartEventType a owl:ObjectProperty ;
    rdfs:label "has start event type" ;
    rdfs:comment "Relation between a state type and an event type. Describes which event type starts a certain state type." ;
    rdfs:domain sense:StateType ;
    rdfs:range sense:EventType .

sense:hosts a owl:ObjectProperty ;
    rdfs:label "hosts" ;
    rdfs:comment "subclass of sosa:hosts -  relation from a Platform to an asset (System or Platform) hosted or mounted on it" ;
    rdfs:domain sense:Platform ;
    rdfs:range sense:Platform,
        sense:Sensor .

sense:MitigationOption a owl:Class ;
    rdfs:label "Mitigation Option" ;
    rdfs:comment "A mitigation option for a state type." .

sense:MitigationPlan a owl:Class ;
    rdfs:label "Mitigation Plan" ;
    rdfs:comment "A mitigation plan for a type of state." .

sense:UserRole a owl:Class ;
    rdfs:label "User Role" ;
    rdfs:comment "User role in terms of access rights. each user has a user role, which allows them access to a part of the system." .

sense:UserType a owl:Class ;
    rdfs:label "User Type" ;
    rdfs:comment "Type of user, in terms of technicality level. Each user has a preferred means of explanation and technicality level, which is defined by this class." .

sense:VirtualSensor a owl:Class ;
    rdfs:label "Virtual Sensor" ;
    rdfs:comment "A sensor, which implicitly collects data about the system. This sensor data is not collected directly, but it can be calculated through a combination of other sensors." ;
    rdfs:subClassOf sense:Sensor .

sense:ObservableProperty a owl:Class ;
    rdfs:label "Observable Property" ;
    rdfs:comment "subclass of sosa:ObservableProperty - identifiable quality of a FeatureOfInterest that can be observed " .

sense:PlatformType a owl:Class ;
    rdfs:label "Platform Type" ;
    rdfs:comment "A type of Platform. Each Platform has a Platform Type." .

sense:StateCausality a owl:Class ;
    rdfs:label "State Causality" ;
    rdfs:comment "A causal relation between two state instances." .

sense:AccessRight a owl:Class ;
    rdfs:label "Access Right" ;
    rdfs:comment "Access Rights, defining access to platforms of the system." .

sense:Event a owl:Class ;
    rdfs:label "Event" ;
    rdfs:comment "something happening in the system, which is of interest. An event is always considered to be happening at a single time point." ;
    owl:disjointWith sense:State .

sense:ParameterBinding a owl:Class ;
    rdfs:label "Parameter Binding" ;
    rdfs:comment "A parameter binding connects parameters from the EventDetection's definition to a literal or a sensor. Examples of parameters are the variables in a formula." .

sense:User a owl:Class ;
    rdfs:label "User" ;
    rdfs:comment "A system user, who requires explanations." .

sense:EventDetection a owl:Class ;
    rdfs:label "Event Detection" ;
    rdfs:comment "A procedure to detect an event in the system. The method of this procedure defines which event specification method is used. The definition of a procedure defines the exact conditions for detecting an event and is formulated according to the method employed." .

sense:Explanation a owl:Class ;
    rdfs:label "Explanation" ;
    rdfs:comment "A user-centered, actionable explanation, designed for a specific user, explaining the root cause of a specific state." .

sense:Observation a owl:Class ;
    rdfs:label "Observation" ;
    rdfs:comment "subclass of sosa:Observation - act of carrying out an ObservingProcedure using a Sensor to estimate or calculate a value of an observable Property of a FeatureOfInterest" .

sense:StateTypeCausality a owl:Class ;
    rdfs:label "State Type Causality" ;
    rdfs:comment "A type causality relation between two state types." .

sense:Platform a owl:Class ;
    rdfs:label "Platform" ;
    rdfs:comment "subclass of sosa:Plaform - entity that hosts other entities, particularly Systems, and other Platforms." .

sense:State a owl:Class ;
    rdfs:label "State" ;
    rdfs:comment "A state of a sensor. A state is a condition of a sensor over a period of time. A state is started and ended by an event." .

sense:EventType a owl:Class ;
    rdfs:label "Event Type" ;
    rdfs:comment "A type of event. Each event has an event type." ;
    owl:disjointWith sense:StateType .

sense:Sensor a owl:Class ;
    rdfs:label "Sensor" ;
    rdfs:comment "subclass of sosa:Sensor - System that implements an ObservingProcedure to determine the value of an observable Property" .

sense:StateType a owl:Class ;
    rdfs:label "State Type" ;
    rdfs:comment "A type of a state. Each state has a state type." .

